WIP: pf_certify exists for a consistent thread

src/prop/PFCertify.v
@@ -25,6 +25,22 @@ Require Import Thread.
 Section PFCertify.
   Variable lang: language.
 
+  Variant certify (reserved: OptTimeMap.t) (loc: Loc.t) (th: Thread.t lang): Prop :=
+    | certify_failure
+        pf e th1 th2
+        (STEPS: rtc (Thread.tau_step reserved) th th1)
+        (STEP_FAILURE: Thread.step reserved pf e th1 th2)
+        (EVENT_FAILURE: ThreadEvent.get_machine_event e = MachineEvent.failure)
+    | certify_fulfill
+        pf e th1 th2
+        from to val released ord
+        (STEPS: rtc (Thread.tau_step reserved) th th1)
+        (STEP_FULFILL: Thread.step reserved pf e th1 th2)
+        (EVENT_FULFILL: ThreadEvent.is_writing e = Some (loc, from, to, val, released, ord))
+        (TO: Time.lt (Memory.max_ts loc (Global.memory (Thread.global th1))) to)
+        (ORD: Ordering.le ord Ordering.na)
+  .
+
   Variant pf_certify (loc: Loc.t) (th: Thread.t lang): Prop :=
     | pf_certify_failure
         pf e th1 th2
@@ -41,11 +57,103 @@ Section PFCertify.
         (ORD: Ordering.le ord Ordering.na)
   .
 
+  Lemma consistent_certify
+        th loc
+        (LC_WF: Local.wf (Thread.local th) (Thread.global th))
+        (GL_WF: Global.wf (Thread.global th))
+        (CONS: Thread.consistent th)
+        (PROMISED: Local.promises (Thread.local th) loc = true):
+    certify (Global.max_reserved (Thread.global th)) loc th.
+  Proof.
+    inv CONS.
+    { inv FAILURE. econs 1; eauto. }
+    remember (Global.max_reserved (Thread.global th)) as reserved.
+    clear Heqreserved. revert PROMISED.
+    induction STEPS; i.
+    { rewrite PROMISES in *. ss. }
+    destruct (Local.promises (Thread.local y) loc) eqn:PROMISEDY.
+    { dup H. inv H0. inv TSTEP.
+      exploit Thread.step_future; try exact STEP; eauto. i. des.
+      exploit IHSTEPS; eauto. i. inv x1.
+      - econs 1; try exact STEP_FAILURE; eauto.
+      - econs 2; try exact STEP_FULFILL; eauto.
+    }
+
+    move PROMISEDY at bottom.
+    inv H. inv TSTEP.
+    inv STEP; inv STEP0; ss; (try congr); (try by inv LOCAL; ss; congr).
+    { (* promise *)
+      inv LOCAL. inv PROMISE. ss.
+      exploit BoolMap.add_le; try exact ADD; eauto. i. congr.
+    }
+
+    { (* write *)
+      assert (loc0 = loc /\ Ordering.le ord Ordering.na).
+      { inv LOCAL. inv FULFILL; ss; try congr. split; ss.
+        revert PROMISEDY. erewrite BoolMap.remove_o; eauto.
+        condtac; ss. congr.
+      }
+      des. subst.
+      destruct (TimeFacts.le_lt_dec to (Memory.max_ts loc (Global.memory gl1))); cycle 1.
+      { econs 2; [refl|..].
+        - econs 2; [|econs 3]; eauto.
+        - ss.
+        - ss.
+        - ss.
+      }
+
+      exploit (Memory.max_ts_spec loc); try apply GL_WF. i. des.
+      destruct msg. clear MAX.
+      econs 1; [refl|..].
+      - econs 2; [|econs 9]; eauto.
+        econs. econs 2; eauto.
+        + unfold TView.racy_view.
+          eapply TimeFacts.lt_le_lt; eauto.
+          inv LOCAL. inv WRITABLE. ss.
+          eapply TimeFacts.le_lt_lt; eauto.
+          apply LC_WF.
+        + destruct ord; ss.
+      - ss.
+    }
+
+    { (* update *)
+      assert (Ordering.le ordw Ordering.na).
+      { inv LOCAL1. inv LOCAL2.  inv FULFILL; ss; try congr. }
+      econs 1; [refl|..].
+      - econs 2; [|econs 10]; eauto.
+      - ss.
+    }
+  Qed.
+
+  Variant sim_thread (th_src th_tgt: Thread.t lang): Prop :=
+    | sim_thread_intro
+        (STATE: Thread.state th_src = Thread.state th_tgt)
+        (TVIEW: Local.tview (Thread.local th_src) = Local.tview (Thread.local th_tgt))
+        (SC: Global.sc (Thread.global th_src) = Global.sc (Thread.global th_tgt))
+        (PROMISES: BoolMap.minus (Global.promises (Thread.global th_src)) (Local.promises (Thread.local th_src)) =
+                   BoolMap.minus (Global.promises (Thread.global th_tgt)) (Local.promises (Thread.local th_tgt)))
+        (RESERVES: BoolMap.minus (Global.reserves (Thread.global th_src)) (Local.reserves (Thread.local th_src)) =
+                   BoolMap.minus (Global.reserves (Thread.global th_tgt)) (Local.reserves (Thread.local th_tgt)))
+        (MEMORY: Global.memory (Thread.global th_src) = Global.memory (Thread.global th_tgt))
+  .
+
+  Lemma certify_pf_certify
+        th loc
+        (LC_WF: Local.wf (Thread.local th) (Thread.global th))
+        (GL_WF: Global.wf (Thread.global th))
+        (CERTIFY: certify (Global.max_reserved (Thread.global th)) loc th):
+    pf_certify loc th.
+  Proof.
+  Admitted.
+
   Lemma consistent_pf_certify
         th loc
+        (LC_WF: Local.wf (Thread.local th) (Thread.global th))
+        (GL_WF: Global.wf (Thread.global th))
         (CONS: Thread.consistent th)
         (PROMISED: th.(Thread.local).(Local.promises) loc = true):
     pf_certify loc th.
   Proof.
-  Admitted.
+    eauto using consistent_certify, certify_pf_certify.
+  Qed.
 End PFCertify.
